theories/MaxOfTwoNumbers/Computed/AllMaskedAttnScores.v
@@ -1,0 +1,22 @@
+From NeuralNetInterp.MaxOfTwoNumbers Require Import Model.
+From NeuralNetInterp.Torch Require Import Tensor.
+From NeuralNetInterp.Util Require Import Pointed ValueExtraction.
+
+Local Notation prea := (masked_attn_scores all_tokens) (only parsing).
+Local Notation prev := (PArray.concretize prea) (only parsing).
+Local Definition pre := prev.
+
+Set NativeCompute Timing.
+Time Local Definition all_tokens_masked_attn_scores_concrete_value := native_compute pre.
+
+Time Definition all_tokens_masked_attn_scores_concrete : PArray.concrete_tensor _ _ := (*Eval native_compute in pre *)Eval hnf in extract all_tokens_masked_attn_scores_concrete_value.
+Time Definition all_tokens_masked_attn_scores_concrete_eq : all_tokens_masked_attn_scores_concrete = prev := extract_eq all_tokens_masked_attn_scores_concrete_value. (*
+Proof. native_cast_no_check (eq_refl prev). Time Qed.*)
+
+Definition all_tokens_masked_attn_scores : tensor _ _ := PArray.reabstract (fun _ => prea) all_tokens_masked_attn_scores_concrete.
+Lemma all_tokens_masked_attn_scores_eq idxs : all_tokens_masked_attn_scores idxs = prea idxs.
+Proof.
+  cbv [all_tokens_masked_attn_scores].
+  erewrite PArray.reabstract_ext_correct by exact all_tokens_masked_attn_scores_concrete_eq.
+  reflexivity.
+Qed.
