theories/Util/List/Instances/NthError.v
@@ -1,0 +1,14 @@
+From Coq Require Import List Morphisms.
+From NeuralNetInterp.Util Require Import Option.
+Import ListNotations.
+#[local] Open Scope list_scope.
+
+Module List.
+  #[export] Instance nth_error_Proper_Forall2 {A R}
+  : Proper (Forall2 R ==> eq ==> option_eq R) (@nth_error A).
+  Proof.
+    intros ?? H n ? <-; revert n.
+    now induction H, n; cbn.
+  Qed.
+End List.
+Export (hints) List.
